Simplify: Remove unop

Imp/Expr/Basic.lean
@@ -1,10 +1,4 @@
-namespace Imp.Expr
-
-/-- Unary operators -/
-inductive UnOp where
-  | neg
-  | not
-deriving Repr, DecidableEq
+namespace Imp
 
 /-- Binary operators -/
 inductive BinOp where
@@ -15,14 +9,9 @@ inductive BinOp where
   | lt | le | eq
 deriving Repr, DecidableEq
 
-end Expr
--- The `Expr` namespace is ended here to avoid doubly-nesting the namespace for the constructors of
--- the `Expr` datatype
-
 /-- Expressions -/
 inductive Expr where
   | const (i : BitVec 32)
   | var (name : String)
-  | un (op : Expr.UnOp) (e : Expr)
-  | bin (op : Expr.BinOp) (e1 e2 : Expr)
+  | op (op : BinOp) (e1 e2 : Expr)
 deriving Repr, DecidableEq
